Switch to our representation of MST

state/IFC.Heap.ST.fst
@@ -4,6 +4,7 @@ open FStar.Tactics
 open FStar.Set
 open FStar.Preorder
 open Monotonic.IFC.Heap
+open MST
 
 module W = FStar.Monotonic.Witnessed
 
@@ -22,29 +23,88 @@ let lheap_rel (h1:lheap) (h2:lheap) =
 
 type lheap_predicate = lheap -> Type0
 
-new_effect GST = STATE_h lheap
+let heap_state : tstate = { t = lheap; rel = lheap_rel }
 
-let gst_pre           = st_pre_h lheap
-let gst_post' (a:Type) (pre:Type) = st_post_h' lheap a pre
-let gst_post  (a:Type) = st_post_h lheap a
-let gst_wp (a:Type)   = st_wp_h lheap a
+let stable (p:lheap_predicate) = stable p heap_state.rel
 
-unfold let lift_div_gst (a:Type) (wp:pure_wp a) (p:gst_post a) (h:lheap) = wp (fun a -> p a h)
-sub_effect DIV ~> GST = lift_div_gst
+let _mst a wp = mst heap_state a wp
+let _mst_bind a b wp_v wp_f v f = mst_bind #heap_state #a #b #wp_v #wp_f v f
+let _mst_return a x = mst_return #heap_state #a x
 
-let stable (p:lheap_predicate) =
-  forall (h1:lheap) (h2:lheap). (p h1 /\ lheap_rel h1 h2) ==> p h2
+let _mst_subcomp a (wp1:st_wp heap_state.t a) (wp2:st_wp heap_state.t a) v:
+  Pure (_mst a wp2) (requires (wp1 ⊑ wp2)) (ensures (fun _ -> True)) = 
+  mst_subcomp #heap_state #a #wp1 #wp2 v
+
+let _mst_if_then_else (a : Type u#a)
+  (#wp1 : st_wp heap_state.t a)
+  (#wp2 : st_wp heap_state.t a)
+  (f : _mst a wp1) (g : _mst a wp2) (b : bool) : Type =
+  _mst a (st_if_then_else heap_state.t a b wp1 wp2)
+
+
+reifiable
+reflectable
+effect {
+  STATEwp (a:Type) (wp : st_wp heap_state.t a)
+  with {
+       repr       = _mst
+     ; return     = _mst_return
+     ; bind       = _mst_bind
+     ; subcomp    = _mst_subcomp
+     ; if_then_else = _mst_if_then_else
+     }
+}
+
+unfold
+let wp_lift_pure_st (w : pure_wp 'a) : st_wp heap_state.t 'a =
+  FStar.Monotonic.Pure.elim_pure_wp_monotonicity_forall ();
+  fun p h -> w (fun r -> p r h)
+
+val lift_pure_mst :
+  a: Type u#a ->
+  w: pure_wp a ->
+  f: (eqtype_as_type unit -> PURE a w) ->
+  Tot (_mst a (wp_lift_pure_st w))
+let lift_pure_mst a w f =
+  FStar.Monotonic.Pure.elim_pure_wp_monotonicity_forall ();
+  let lhs = partial_return heap_state (as_requires w) in
+  let rhs = (fun (pre:(squash (as_requires w))) -> _mst_return a (f pre)) in
+  let m = _mst_bind _ _ _ _ lhs rhs in
+  _mst_subcomp _ _ _ m
+
+sub_effect PURE ~> STATEwp = lift_pure_mst
+
+private
+let _get () : STATEwp lheap get_wp = 
+  STATEwp?.reflect (mst_get ())
+
+private
+let _put (h1:lheap) : STATEwp unit (put_wp h1) = 
+  STATEwp?.reflect (mst_put h1)
+
+type heap_predicate = lheap -> Type0
 
 [@@"opaque_to_smt"]
-let witnessed (p:lheap_predicate) = W.witnessed lheap_rel p
+let witnessed (pred:heap_predicate{stable pred}) : Type0 = W.witnessed heap_state.rel pred
 
-private
-assume val gst_get: unit    -> GST lheap (fun p h0 -> p h0 h0)
-private
-assume val gst_put: h1:lheap -> GST unit (fun p h0 -> lheap_rel h0 h1 /\ p () h1)
+let mst_witness (pred:heap_predicate) : STATEwp unit (fun p h -> pred h /\ stable pred /\ (witnessed pred ==> p () h)) = 
+  STATEwp?.reflect (mst_witness pred)
 
-assume val gst_witness: p:lheap_predicate -> GST unit (fun post h0 -> p h0 /\ stable p /\ (witnessed p ==> post () h0))
-assume val gst_recall:  p:lheap_predicate -> GST unit (fun post h0 -> witnessed p /\ (p h0 ==> post () h0))
+let mst_recall (pred:heap_predicate{stable pred}) : STATEwp unit (fun p h -> witnessed pred /\ (pred h ==> p () h)) = 
+  STATEwp?.reflect (mst_recall pred)
+
+(** *** From here it is mostly a COPY-PASTE from FStar.ST **)
+let st_pre           = st_pre_h lheap
+let st_post' (a:Type) (pre:Type) = st_post_h' lheap a pre
+let st_post  (a:Type) = st_post_h lheap a
+let st_wp (a:Type)   = st_wp_h lheap a
+
+effect ST (a:Type) (pre:st_pre) (post: (h:lheap -> Tot (st_post' a (pre h)))) =
+  STATEwp a (fun (p:st_post a) (h:lheap) -> pre h /\ (forall a h1. h `lheap_rel` h1 /\ post h a h1 ==> p a h1))
+effect St (a:Type) = ST a (fun h -> True) (fun h0 r h1 -> True)
+
+// unfold let lift_div_gst (a:Type) (wp:pure_wp a) (p:gst_post a) (h:lheap) = wp (fun a -> p a h)
+// sub_effect DIV ~> GST = lift_div_gst
 
 val lemma_functoriality (p:lheap_predicate{stable p /\ witnessed p}) 
                         (q:lheap_predicate{stable q /\ (forall (h:lheap). p h ==> q h)})
@@ -53,29 +113,10 @@ let lemma_functoriality p q =
   reveal_opaque (`%witnessed) witnessed;
   W.lemma_witnessed_weakening lheap_rel p q
 
-let st_pre   = gst_pre
-let st_post' = gst_post'
-let st_post  = gst_post
-let st_wp    = gst_wp
-
-new_effect STATE = GST
-
-unfold let lift_gst_state (a:Type) (wp:gst_wp a) = wp
-sub_effect GST ~> STATE = lift_gst_state
-
-effect State (a:Type) (wp:st_wp a) = STATE a wp
-
-effect ST (a:Type) (pre:st_pre) (post: (h:lheap -> Tot (st_post' a (pre h)))) =
-  STATE a (fun (p:st_post a) (h:lheap) -> pre h /\ (forall a h1. h `lheap_rel` h1 /\ post h a h1 ==> p a h1))
-effect St (a:Type) = ST a (fun h -> True) (fun h0 r h1 -> True)
-
-let contains_pred (#a:Type0) (#rel:preorder a) (r:mref a rel) = fun lh -> lh `contains` r
+let contains_pred (#a:Type0) (#rel:preorder a) (r:mref a rel) = fun lh -> lh `contains` r /\ is_mm r = false
 
 let contains_stable (#a:Type0) (#rel:preorder a) (r:mref a rel) : Lemma (stable (contains_pred r)) 
-  [SMTPat (contains_pred r)]=
-  assert (stable (contains_pred r)) by (
-    norm [delta_only [`%stable;`%lheap_rel]; iota]
-  )
+  [SMTPat (contains_pred r)] by (unfold_def (`stable)) = ()
 
 type mref (a:Type0) (rel:preorder a) = 
   mref a rel
@@ -91,14 +132,14 @@ let alloc_post (#a:Type) (#rel:preorder a) (init:a) (h0:lheap) (r:mref a rel) (h
 
 let alloc (#a:Type) (#rel:preorder a) (init:a)
 : ST (mref a rel) (fun h -> True) (alloc_post #a #rel init)
-= let h0 = gst_get () in
+= let h0 = _get () in
   let r, h1 = alloc rel h0 init false in
   assert (lheap_rel h0 h1) by (norm [delta_only [`%lheap_rel]; iota]);
-  gst_put h1;
+  _put h1;
   r
 
-let read (#a:Type) (#rel:preorder a) (r:mref a rel) : STATE a (fun p h -> contains_pred r h /\ p (sel h r) h)
-= let h0 = gst_get () in
+let read (#a:Type) (#rel:preorder a) (r:mref a rel) : STATEwp a (fun p h -> contains_pred r h /\ p (sel h r) h)
+= let h0 = _get () in
   lemma_sel_equals_sel_tot_for_contained_refs h0 r;
   sel_tot h0 r    
 
@@ -116,13 +157,13 @@ let write (#a:Type) (#rel:preorder a) (r:mref a rel) (v:a)
 : ST unit
   (fun h -> contains_pred r h /\ rel (sel h r) v)
   (write_post #a #rel r v)
-= let h0 = gst_get () in
+= let h0 = _get () in
   let h1 = upd_tot h0 r v in
   lemma_distinct_addrs_distinct_preorders ();
   lemma_distinct_addrs_distinct_mm ();
   lemma_upd_equals_upd_tot_for_contained_refs h0 r v;
   assert (lheap_rel h0 h1) by (norm [delta_only [`%lheap_rel]; iota]);
-  gst_put h1
+  _put h1
 
 let modifies_none (h0:lheap) (h1:lheap) = modifies Set.empty h0 h1
 
@@ -138,14 +179,14 @@ let declassify (#a:Type) (#rel:preorder a) (r:mref a rel) (l:label)
   (fun h -> contains_pred r h /\ label_of r h `label_gte` l)
   (declassify_post #a #rel r l)
 =
-  let h0 = gst_get () in
+  let h0 = _get () in
   let h1 = declassify_tot #a #rel h0 l r in
   assert (lheap_rel h0 h1) by (norm [delta_only [`%lheap_rel]; iota]);
-  gst_put h1
+  _put h1
 
 
 let op_Bang (#a:Type) (#rel:preorder a) (r:mref a rel)
-  : STATE a (fun p h -> contains_pred r h /\ p (sel h r) h)
+  : STATEwp a (fun p h -> contains_pred r h /\ p (sel h r) h)
 = read #a #rel r
 
 let op_Colon_Equals (#a:Type) (#rel:preorder a) (r:mref a rel) (v:a)
@@ -157,15 +198,12 @@ let op_Colon_Equals (#a:Type) (#rel:preorder a) (r:mref a rel) (v:a)
 type ref (a:Type0) = mref a (FStar.Heap.trivial_preorder a)
 
 let get (u:unit) :ST (FStar.Ghost.erased lheap) (fun h -> True) (fun h0 h h1 -> h0==h1 /\ (FStar.Ghost.reveal h)==h1) =
-  gst_get ()
+  _get ()
 
-let is_low_pred (#a:Type0) (r:ref a) = fun lh -> lh `contains` r /\ label_of r lh == Low
+let is_low_pred (#a:Type0) (#rel:preorder a) (r:mref a rel) = fun h -> contains_pred r h /\ label_of r h == Low
 
 let is_low_pred_stable (#a:Type0) (r:ref a) : Lemma (stable (is_low_pred r))
-  [SMTPat (is_low_pred r)] =  
-  assert (stable (is_low_pred r)) by (
-    norm [delta_only [`%stable;`%lheap_rel]; iota]
-  )
+  [SMTPat (is_low_pred r)] by (unfold_def (`stable)) = ()
 
 let declassify_low (#a:Type) (r:ref a)
 : ST (ref a)
@@ -183,8 +221,12 @@ let declassify_low (#a:Type) (r:ref a)
 val lemma_modifies_only_label_trans
    (l:label) (h0 h1 h2:lheap)
    : Lemma
-     (requires equal_ll h0 h1 /\ lheap_rel h0 h1 /\ lheap_rel h1 h2 /\
-     modifies_only_label l h0 h1 /\ modifies_only_label l h1 h2)
+     (requires 
+      modifies_classification Set.empty h0 h1 /\ 
+      lheap_rel h0 h1 /\ 
+      lheap_rel h1 h2 /\
+      modifies_only_label l h0 h1 /\ 
+      modifies_only_label l h1 h2)
      (ensures modifies_only_label l h0 h2)
  //  [SMTPat (modifies_only_label l h0 h1); SMTPat (modifies_only_label l h1 h2)]
 let lemma_modifies_only_label_trans l h0 h1 h2 = 
